src/verilog/Verilog.v
@@ -713,6 +713,8 @@ Definition empty_stack (m : module) : assocmap_arr :=
 Inductive step : genv -> state -> Events.trace -> state -> Prop :=
   | step_module :
       forall asr asa asr' asa' basr1 nasr1 basa1 nasa1 f stval pstval m sf st g,
+      asr!(m.(mod_st)) = Some ist ->
+      valueToPos ist = st ->
       mis_stepp f (mkassociations asr empty_assocmap)
                   (mkassociations asa (empty_stack m))
                   m.(mod_body)
